specs/SMRAMC.v
@@ -1,5 +1,3 @@
-Require Import FreeSpec.Libs.Vector.Vector.
-Require Import FreeSpec.Specs.Hexa.
 Require Import FreeSpec.Specs.Memory.
 Require Import Coq.Program.Program.
 Require Import Omega.
@@ -7,66 +5,26 @@ Require Import Omega.
 Definition SMRAMC : Type := byte.
 
 Definition SMRAMC_C_BASE_SEG : Type := mem 3.
-Definition SMRAMC_D_LCK : Type := bit.
-Definition SMRAMC_D_CLS : Type := bit.
-Definition SMRAMC_D_OPEN : Type := bit.
+Definition SMRAMC_D_LCK : Type := mem 1.
+Definition SMRAMC_D_CLS : Type := mem 1.
+Definition SMRAMC_D_OPEN : Type := mem 1.
 
-Program Definition read_c_base_seg
-        (reg: SMRAMC)
-  : { f: SMRAMC_C_BASE_SEG | forall i, i < 3 -> nth f i = nth reg i } :=
-  take reg 3.
-Next Obligation.
-  repeat apply le_n_S.
-  assert (forall i, 0 <= i). {
-    induction i.
-    constructor.
-    apply le_S.
-    exact IHi.
-  }
-  apply H.
-Defined.
+Definition read_c_base_seg
+           (reg: SMRAMC)
+  : SMRAMC_C_BASE_SEG :=
+  cast 3 reg.
 
 Program Definition read_d_lck
         (reg: SMRAMC)
-  : { f: SMRAMC_D_LCK | Some f = nth reg 4 } :=
-  head (extract reg 5 4).
-Next Obligation.
-  destruct head.
-  destruct take.
-  destruct drop.
-  cbn in *.
-  rewrite <- e1; [| omega ].
-  rewrite <- e0; [| omega].
-  symmetry.
-  exact e.
-Defined.
+  : SMRAMC_D_LCK :=
+  cast 1 (shiftr reg 4).
 
 Program Definition read_d_cls
         (reg: SMRAMC)
-  : { f: SMRAMC_D_LCK | Some f = nth reg 5 } :=
-  head (extract reg 6 5).
-Next Obligation.
-  destruct head.
-  destruct take.
-  destruct drop.
-  cbn in *.
-  rewrite <- e1; [| omega ].
-  rewrite <- e0; [| omega].
-  symmetry.
-  exact e.
-Defined.
+  : SMRAMC_D_LCK :=
+  cast 1 (shiftr reg 5).
 
 Program Definition read_d_open
         (reg: SMRAMC)
-  : { f: SMRAMC_D_OPEN | Some f = nth reg 6 } :=
-  head (extract reg 7 6).
-Next Obligation.
-  destruct head.
-  destruct take.
-  destruct drop.
-  cbn in *.
-  rewrite <- e1; [| omega ].
-  rewrite <- e0; [| omega].
-  symmetry.
-  exact e.
-Defined.
+  : SMRAMC_D_OPEN :=
+  cast 1 (shiftr reg 6).
